examples/containers/theories/SetProofs.v
@@ -1,6 +1,8 @@
 Require Import GHC.Base.
+Require Import Data.Semigroup.
 Import GHC.Base.Notations.
 Require Import Proofs.GHC.Base.
+Require Proofs.Data.Foldable.
 Require Import Data.Set.Internal.
 Import GHC.Num.Notations.
 Require Import OrdTactic.
@@ -688,6 +690,30 @@ Proof.
   all: try solve [solve_Desc].
 Qed.
 
+Lemma balanceL_noop :
+    forall x s1 s2 lb ub,
+    Bounded s1 lb (Some x) ->
+    Bounded s2 (Some x) ub ->
+    isLB lb x = true ->
+    isUB ub x = true->
+    balance_prop (size s1) (size s2) ->
+    balanceL x s1 s2 = Bin (1 + size s1 + size s2) x s1 s2.
+Proof.
+  intros.
+
+  unfold balanceL.
+  unfold op_zg__, op_zl__, Ord_Integer___, op_zg____, op_zl____.
+
+  repeat lazymatch goal with [ H : Bounded ?s _ _ |- context [match ?s with _ => _ end] ] => inversion H; subst; clear H end;
+  repeat lazymatch goal with [ |- context [if (?x <? ?y)%Z then _ else _] ] => destruct (Z.ltb_spec x y) end;
+  rewrite ?size_Bin in *; simpl (size Tip) in *; simpl sem;
+  simpl isLB in *;
+  simpl isUB in *.
+  all: try solve [exfalso; lia_sizes]. (* Some are simply impossible *)
+  all: repeat find_Tip.
+  all: try reflexivity.
+Qed.
+
 (** *** Verification of [balanceR] *)
 
 Lemma balanceR_Desc:
@@ -715,6 +741,31 @@ Proof.
   all: repeat find_Tip.
   all: try solve [solve_Desc].
 Qed.
+
+Lemma balanceR_noop :
+    forall x s1 s2 lb ub,
+    Bounded s1 lb (Some x) ->
+    Bounded s2 (Some x) ub ->
+    isLB lb x = true ->
+    isUB ub x = true->
+    balance_prop (size s1) (size s2) ->
+    balanceR x s1 s2 = Bin (1 + size s1 + size s2) x s1 s2.
+Proof.
+  intros.
+
+  unfold balanceR.
+  unfold op_zg__, op_zl__, Ord_Integer___, op_zg____, op_zl____.
+
+  repeat lazymatch goal with [ H : Bounded ?s _ _ |- context [match ?s with _ => _ end] ] => inversion H; subst; clear H end;
+  repeat lazymatch goal with [ |- context [if (?x <? ?y)%Z then _ else _] ] => destruct (Z.ltb_spec x y) end;
+  rewrite ?size_Bin in *; simpl (size Tip) in *; simpl sem;
+  simpl isLB in *;
+  simpl isUB in *.
+  all: try solve [exfalso; lia_sizes]. (* Some are simply impossible *)
+  all: repeat find_Tip.
+  all: try reflexivity.
+Qed.
+
 
 (** *** Verification of [insertMax] *)
 
@@ -843,6 +894,17 @@ Proof.
       rewrite (sem_outside_above HB1) by order_Bounds.
       rewrite orb_false_l.
       reflexivity.
+Qed.
+
+(** ** Verification of [notMember] *)
+
+Lemma notMember_spec:
+ forall {s lb ub i}, Bounded s lb ub -> notMember i s = negb (sem s i).
+Proof.
+  intros ???? HB.
+  unfold notMember, op_zd__.
+  erewrite member_spec by eassumption.
+  reflexivity.
 Qed.
 
 
@@ -1057,6 +1119,130 @@ Proof.
     split; [left; reflexivity | solve_Desc].
 Qed.
 
+(** ** Verification of [lookupMin] *)
+
+Lemma lookupMinSure_Desc:
+  forall s x lb ub,
+    Bounded s lb ub ->
+    let y := lookupMinSure x s in
+    ((forall i, sem s i = false) /\ y = x \/
+     sem s y = true /\ (forall i, sem s i = true -> (y GHC.Base.<= i) = true)).
+Proof.
+  intros ???? HD. revert x.
+  induction HD. intro x.
+  * left. simpl. intuition.
+  * right. clear IHHD2.
+    simpl.
+    destruct (IHHD1 x) as [[??]|[??]]; clear IHHD1.
+    - rewrite H4. clear H4.
+      setoid_rewrite H3. clear H3.
+      rewrite Eq_refl. split; only 1: reflexivity.
+      intros i Hi.
+      rewrite orb_false_l in *.
+      rewrite orb_true_iff in Hi. destruct Hi.
+      + order_Bounds.
+      + repeat (f_solver_step; f_solver_cleanup).
+    - rewrite H3. split; only 1: reflexivity.
+      intros i Hi.
+      rewrite !orb_true_iff in Hi. decompose [or] Hi; clear Hi.
+      + intuition.
+      + repeat (f_solver_step; f_solver_cleanup).
+      + repeat (f_solver_step; f_solver_cleanup).
+Qed.
+
+Lemma lookupMin_Desc:
+  forall s lb ub,
+    Bounded s lb ub ->
+    match lookupMin s with 
+      | None => (forall i, sem s i = false)
+      | Some y => sem s y = true /\ (forall i, sem s i = true -> (y GHC.Base.<= i) = true)
+    end.
+Proof.
+  intros.
+  unfold lookupMin. unfold op_zdzn__.
+  inversion H; subst; clear H.
+  * reflexivity.
+  * simpl.
+    destruct (lookupMinSure_Desc s1 x lb (Some x) H0) as [[??]|[??]].
+    - rewrite H4. clear H4.
+      setoid_rewrite H. clear H.
+      rewrite Eq_refl. split; only 1: reflexivity.
+      intros i Hi.
+      rewrite orb_false_l in *.
+      rewrite orb_true_iff in Hi. destruct Hi.
+      + order_Bounds.
+      + repeat (f_solver_step; f_solver_cleanup).
+    - rewrite H. split; only 1: reflexivity.
+      intros i Hi.
+      rewrite !orb_true_iff in Hi. decompose [or] Hi; clear Hi.
+      + intuition.
+      + repeat (f_solver_step; f_solver_cleanup).
+      + repeat (f_solver_step; f_solver_cleanup).
+Qed.
+
+(** ** Verification of [lookupMax] *)
+
+Lemma lookupMaxSure_Desc:
+  forall s x lb ub,
+    Bounded s lb ub ->
+    let y := lookupMaxSure x s in
+    ((forall i, sem s i = false) /\ y = x \/
+     sem s y = true /\ (forall i, sem s i = true -> (i GHC.Base.<= y) = true)).
+Proof.
+  intros ???? HD. revert x.
+  induction HD. intro x.
+  * left. simpl. intuition.
+  * right. clear IHHD1.
+    simpl.
+    destruct (IHHD2 x) as [[??]|[??]]; clear IHHD2.
+    - rewrite H4. clear H4.
+      setoid_rewrite H3. clear H3.
+      rewrite Eq_refl, !orb_true_r.
+      split; only 1: reflexivity.
+      intros i Hi.
+      rewrite orb_false_r in *.
+      rewrite orb_true_iff in Hi. destruct Hi.
+      + repeat (f_solver_step; f_solver_cleanup).
+      + order_Bounds.
+    - rewrite H3, !orb_true_r. split; only 1: reflexivity.
+      intros i Hi.
+      rewrite !orb_true_iff in Hi. decompose [or] Hi; clear Hi.
+      + repeat (f_solver_step; f_solver_cleanup).
+      + repeat (f_solver_step; f_solver_cleanup).
+      + intuition.
+Qed.
+
+Lemma lookupMax_Desc:
+  forall s lb ub,
+    Bounded s lb ub ->
+    match lookupMax s with 
+      | None => (forall i, sem s i = false)
+      | Some y => sem s y = true /\ (forall i, sem s i = true -> (i GHC.Base.<= y) = true)
+    end.
+Proof.
+  intros.
+  unfold lookupMax. unfold op_zdzn__.
+  inversion H; subst; clear H.
+  * reflexivity.
+  * simpl.
+    destruct (lookupMaxSure_Desc s2 x (Some x) ub H1) as [[??]|[??]].
+    - rewrite H4. clear H4.
+      setoid_rewrite H. clear H.
+      rewrite Eq_refl, orb_true_r. split; only 1: reflexivity.
+      intros i Hi.
+      rewrite orb_false_r in *.
+      rewrite orb_true_iff in Hi. destruct Hi.
+      + repeat (f_solver_step; f_solver_cleanup).
+      + order_Bounds.
+    - rewrite H, !orb_true_r. split; only 1: reflexivity.
+      intros i Hi.
+      rewrite !orb_true_iff in Hi. decompose [or] Hi; clear Hi.
+      + repeat (f_solver_step; f_solver_cleanup).
+      + repeat (f_solver_step; f_solver_cleanup).
+      + intuition.
+Qed.
+
+
 (** ** Verification of [minViewSure] *)
 
 Lemma minViewSure_Desc:
@@ -1156,6 +1342,84 @@ Proof.
         solve_Desc.
       * destruct (sem s2 x); applyDesc balanceL_Desc; solve_Desc.
 Qed.
+
+(** ** Verification of [deleteMin] *)
+
+(** It is hard to phrase this without refering to [lookupMin] *)
+
+Lemma deleteMin_Desc :
+  forall s lb ub,
+  Bounded s lb ub ->
+  deleteMin s = match lookupMin s with | None => s
+                                       | Some x => delete x s end.
+Proof.
+  intros ??? HD.
+  induction HD.
+  * reflexivity.
+  * clear IHHD2.
+    cbn [deleteMin].
+    rewrite IHHD1; clear IHHD1.
+
+    destruct s1 eqn:?.
+    + replace (lookupMin (Bin sz x (Bin s3 e0 s4 s5) s2)) with (lookupMin (Bin s3 e0 s4 s5)) by reflexivity.
+      rewrite <- Heqs in *. clear  s3 e0 s4 s5 Heqs.
+
+      pose proof (lookupMin_Desc s1 lb (Some x) HD1) as Hlookup.
+      destruct (lookupMin s1) as [ex|].
+      - destruct Hlookup as [Hthere Hextrem].
+        simpl.
+        apply (sem_inside HD1) in Hthere. destruct Hthere.
+        replace (compare ex x) with Lt by (symmetry; solve_Bounds).
+        ** destruct_ptrEq.
+           ++ rewrite Hpe. clear Hpe.
+              eapply balanceR_noop; try eassumption.
+           ++ reflexivity.
+       - rewrite H1.
+          eapply balanceR_noop; try eassumption.
+   + simpl.
+     replace (compare x x) with Eq by (symmetry; order e).
+     reflexivity.
+Qed.
+
+
+(** ** Verification of [deleteMax] *)
+
+(** It is hard to phrase this without refering to [lookupMax] *)
+
+Lemma deleteMax_Desc :
+  forall s lb ub,
+  Bounded s lb ub ->
+  deleteMax s = match lookupMax s with | None => s
+                                       | Some x => delete x s end.
+Proof.
+  intros ??? HD.
+  induction HD.
+  * reflexivity.
+  * clear IHHD1.
+    cbn [deleteMax].
+    rewrite IHHD2; clear IHHD2.
+
+    destruct s2 eqn:?.
+    + replace (lookupMax (Bin sz x s1 (Bin s3 e0 s4 s5))) with (lookupMax (Bin s3 e0 s4 s5)) by reflexivity.
+      rewrite <- Heqs in *. clear  s3 e0 s4 s5 Heqs.
+
+      pose proof (lookupMax_Desc s2 (Some x) ub HD2) as Hlookup.
+      destruct (lookupMax s2) as [ex|].
+      - destruct Hlookup as [Hthere Hextrem].
+        simpl.
+        apply (sem_inside HD2) in Hthere. destruct Hthere.
+        replace (compare ex x) with Gt by (symmetry; solve_Bounds).
+        ** destruct_ptrEq.
+           ++ rewrite Hpe. clear Hpe.
+              eapply balanceL_noop; try eassumption.
+           ++ reflexivity.
+       - rewrite H1.
+          eapply balanceL_noop; try eassumption.
+   + simpl.
+     replace (compare x x) with Eq by (symmetry; order e).
+     destruct s1; reflexivity.
+Qed.
+
 
 (** ** Verification of [splitS] *)
 
@@ -1270,6 +1534,46 @@ Proof.
         solve_Desc.
 Qed.
 
+(** ** Verification of [unions] *)
+
+(* This is a bit of a lazy specification, but goes a long way *)
+
+Lemma Forall_rev:
+  forall A P (l : list A), Forall P (rev l) <-> Forall P l.
+Proof. intros. rewrite !Forall_forall. setoid_rewrite <- in_rev. reflexivity. Qed.
+
+Lemma existsb_rev:
+  forall A P (l : list A), existsb P (rev l) = existsb P l.
+Proof. intros. apply eq_iff_eq_true. rewrite !existsb_exists. setoid_rewrite <- in_rev. reflexivity. Qed.
+
+
+
+Lemma unions_Desc:
+  forall ss lb ub,
+  Forall (fun s => Bounded s lb ub) ss ->
+  Desc' (unions ss) lb ub (fun i => existsb (fun s => sem s i) ss).
+Proof.
+  intros.
+  unfold unions.
+  (* Switch to a fold right *)
+  rewrite Proofs.Data.Foldable.hs_coq_foldl_list.
+  rewrite <- fold_left_rev_right.
+  rewrite <- (rev_involutive ss).
+  rewrite <- (rev_involutive ss), Forall_rev in H.
+  generalize dependent (rev ss). intros.
+  rewrite rev_involutive.
+
+  induction H.
+  * simpl. applyDesc empty_Desc. solve_Desc.
+  * simpl fold_right.
+    applyDesc IHForall.
+    applyDesc union_Desc.
+    solve_Desc.
+    intro i.
+    rewrite Hsem0, Hsem.
+    rewrite !existsb_rev.
+    simpl. rewrite orb_comm. reflexivity.
+Qed.
 
 (** ** Verification of [merge] *)
 
@@ -1470,6 +1774,35 @@ Proof.
            (* Small [f_solver] incompleteness. *)
            rewrite Hsem0 in H9.
            repeat (f_solver_cleanup; f_solver_step).
+Qed.
+
+(** ** Verification of [disjoint] *)
+
+Lemma disjoint_Desc:
+  forall s1 s2 lb ub,
+  Bounded s1 lb ub ->
+  Bounded s2 lb ub ->
+  disjoint s1 s2 = true <-> (forall i, sem s1 i && sem s2 i = false).
+Proof.
+  intros ???? HB1 HB2.
+  revert s2 HB2.
+  induction HB1; intros s3 HB3.
+  - intuition.
+  - simpl. destruct s3 eqn:Hs3.
+    + rewrite<- Hs3 in *. clear Hs3 e0 s4 s5 s6.
+      eapply splitMember_Desc;
+        only 1: eassumption.
+      intros s4' b s5' HB1 HB2 Hi.
+      rewrite !andb_true_iff.
+      rewrite IHHB1_1 by assumption; clear IHHB1_1.
+      rewrite IHHB1_2 by assumption; clear IHHB1_2.
+      split;intro Hyp; [decompose [and] Hyp | split; [| split]];
+        try f_solver.
+      * specialize (Hyp x). specialize (Hi x).
+        rewrite Eq_refl in Hi. rewrite Eq_refl in Hyp.
+        rewrite negb_true_iff.
+        repeat f_solver_cleanup.
+    + simpl. setoid_rewrite andb_false_r. intuition.
 Qed.
 
 (** ** Verification of [foldr] *)
@@ -2963,6 +3296,7 @@ Local Ltac unfold_WFSet_Eq :=
   unfold "_==_", "_/=_", Eq_Set_WF => /=;
   unfold "_==_", "_/=_", Eq___Set_ => /=;
   unfold Data.Set.Internal.Eq___Set__op_zsze__, Data.Set.Internal.Eq___Set__op_zeze__ => /=.
+
 Global Instance EqLaws_Set : EqLaws WFSet.
 Proof.
   constructor.
@@ -3051,6 +3385,131 @@ Proof.
   - by move=> a b; rewrite Neq_inv negbK compare_flip; case: (compare _ _).
   - by move=> a b; rewrite !Neq_inv compare_flip; case: (compare _ _).
   - by move=> a b; rewrite Neq_inv negbK compare_flip; case: (compare _ _).
+Qed.
+
+(** ** Verification of [Semigroup] *)
+
+Ltac unfold_Monoid_Set :=
+  unfold mappend, mconcat, mempty, Monoid__Set_, mappend__, mconcat__, mempty__,
+         Internal.Monoid__Set__mappend, Internal.Monoid__Set__mconcat, Internal.Monoid__Set__mempty,
+         Semigroup.op_zlzg__,  Semigroup__Set_, Semigroup.op_zlzg____,
+         Internal.Semigroup__Set__op_zlzg__
+    in *.
+
+Program Instance Semigroup_WF : Semigroup WFSet := fun _ k => k
+  {| op_zlzg____  := @mappend (Set_ e) _ |}.
+Next Obligation.
+  destruct x as [s1 HB1], x0 as [s2 HB2]. simpl.
+  unfold_Monoid_Set.
+  eapply union_Desc; try eassumption. intuition.
+Qed.
+
+
+Global Instance SemigroupLaws_Set : SemigroupLaws WFSet.
+Proof.
+  constructor.
+  intros.
+  destruct x as [s1 HB1], y as [s2 HB2], z as [s3 HB3].
+  unfold op_zeze__, Eq_Set_WF, op_zeze____,  proj1_sig.
+  unfold op_zlzg__, Semigroup_WF, op_zlzg____.
+  unfold mappend, Monoid__Set_, mappend__.
+  unfold Internal.Monoid__Set__mappend.
+  unfold proj1_sig.
+  unfold op_zlzg__, Semigroup__Set_, op_zlzg____.
+  unfold Internal.Semigroup__Set__op_zlzg__.
+  eapply (union_Desc s1 s2); try eassumption. intros s12 Hs12 _ Hsem12.
+  eapply (union_Desc s2 s3); try eassumption. intros s23 Hs23 _ Hsem23.
+  eapply (union_Desc s1 s23); try eassumption. intros s1_23 Hs1_23 _ Hsem1_23.
+  eapply (union_Desc s12 s3); try eassumption. intros s12_3 Hs12_3 _ Hsem12_3.
+  rewrite -> equals_spec by eassumption.
+  intro i. rewrite Hsem12_3  Hsem1_23 Hsem23  Hsem12.
+  rewrite orb_assoc. reflexivity.
+Qed.
+
+(** ** Verification of [Monoid] *)
+
+Program Instance Monoid_WF : Monoid WFSet := fun _ k => k
+  {| mempty__   := @mempty (Set_ e) _
+   ; mappend__  := @mappend (Set_ e) _
+   ; mconcat__  xs := @mconcat (Set_ e) _ (List.map (fun x => proj1_sig x) xs)
+  |}.
+Next Obligation.
+  destruct x as [s1 HB1], x0 as [s2 HB2]. simpl.
+  unfold_Monoid_Set.
+  eapply union_Desc; try eassumption. intuition.
+Qed.
+Next Obligation.
+  unfold_Monoid_Set.
+  eapply unions_Desc.
+  * induction xs.
+    + constructor.
+    + destruct a as [s HB]. simpl. constructor. apply HB. apply IHxs.
+  * intros. assumption.
+Qed.
+Next Obligation.
+  unfold_Monoid_Set.
+  eapply empty_Desc.
+  eauto.
+Qed.
+
+Lemma unions_foldr_union:
+  forall (ss : list (Set_ e)),
+  Forall WF ss -> (unions ss == Base.foldr union empty ss) = true.
+Proof.
+  intros.
+  assert (Desc' (Base.foldr union empty ss) None None (fun i => existsb (fun s => sem s i) ss)). {
+    induction H.
+    * simpl. eapply empty_Desc; intros. apply showDesc'. eauto.
+    * simpl.
+      apply IHForall. intros.
+      eapply union_Desc; try eassumption; intros.
+      apply showDesc'. intuition. rewrite H6 H3. reflexivity.
+  }
+  eapply H0. intros.
+  eapply unions_Desc; try eassumption; intros.
+  rewrite -> equals_spec by eassumption.
+  intro i. rewrite H6 H3. reflexivity.
+Qed.
+
+Global Instance MonoidLaws_Set : MonoidLaws WFSet.
+Proof.
+  constructor;
+    unfold op_zeze__, Eq_Set_WF, op_zeze____,  proj1_sig;
+    repeat unfold mappend, mconcat, mempty, Monoid_WF, mappend__, mconcat__, mempty__,
+      Internal.Monoid__Set__mappend, Internal.Monoid__Set__mempty,
+      Semigroup.op_zlzg__,  Semigroup__Set_, Semigroup_WF, Semigroup.op_zlzg____,
+      Internal.Semigroup__Set__op_zlzg__,
+      mappend, mempty, Monoid__Set_, mappend__, mempty__,
+      Internal.Monoid__Set__mappend, Internal.Monoid__Set__mempty, Internal.Monoid__Set__mconcat.
+  * intros. destruct x as [s Hs]; unfold proj1_sig.
+    eapply empty_Desc. intros.
+    eapply union_Desc; try eassumption; intros.
+    rewrite -> equals_spec by eassumption.
+    intro i. rewrite H4 H1. reflexivity.
+  * intros. destruct x as [s Hs]; unfold proj1_sig.
+    eapply empty_Desc. intros.
+    eapply union_Desc; try eassumption; intros.
+    rewrite -> equals_spec by eassumption.
+    intro i. rewrite H4 H1. rewrite orb_false_r. reflexivity.
+  * intros. destruct x as [s1 Hs1], y as [s2 Hs2]; unfold proj1_sig.
+    eapply union_Desc; try eassumption; intros.
+    rewrite -> equals_spec by eassumption.
+    reflexivity.
+  * intros.
+    rename x into xs.
+    lazymatch goal with |- (_ == ?y) = true  =>
+      replace y with (Base.foldr union  empty (List.map (fun x => proj1_sig x) xs))
+    end.
+    + apply unions_foldr_union.
+      induction xs.
+      - constructor.
+      - destruct a as [s Hs]; unfold proj1_sig.
+        constructor; assumption.
+    + induction xs.
+      - reflexivity.
+      - simpl in *.
+        f_equal.
+        assumption.
 Qed.
 
 End TypeClassLaws.
